# Lesson 1 - Recursion
## Lesson Description
Looking into the actual inspection of several different recursion method implementations.  Each implementation will break down the recursion tree depth to determine the actual expected result.

## Problems
### Problem 1
>
```java
public static int f1(int N) {
    if (N < 0) return 0;
    if (N == 0) return 1;
    return f1(N-1) + f1(N-2) + f1(N-3);
}
```

#### Desired Outputs
##### f1(3)
>
f1(3)
    -> f1(2)
        -> f1(1)
            -> f1(0)
                <- 1
            -> f1(-1)
                <- 0
            -> f1(-2)
                <- 0
            <- 1 + 0 + 0
        -> f1(0)
            <- 1
        -> f1(-1)
            <- 0 
        <-  (1 + 0 + 0) + 1 + 0
    -> f1(1)
        -> f1(0)
            <- 1
        -> f1(-1)
            <- 0
        -> f1(-2)
            <- 0
        <- 1 + 0 + 0
    -> f1(0)
        <- 1
    <- ((1 + 0 + 0) + 1 + 0) + (1 + 0 + 0) + (1) = 4

##### f1(5)
>
f1(5)
    -> f1(4)
        -> f1(3)
            -> f1(2)
                -> f1(1)
                    -> f1(0)
                        <- 1
                    -> f1(-1)
                        <- 0
                    -> f1(-2)
                        <- 0
                    <- 1 + 0 + 0
                -> f1(0)
                    <- 1
                -> f1(-1)
                    <- 0
                <- (1 + 0 + 0) + 1 + 0
            -> f1(1)
                -> f1(0)
                    <- 1
                -> f1(-1)
                    <- 0
                -> f1(-2)
                    <- 0
                <- 1 + 0 + 0
            -> f1(0)
                <- 1
            <- ((1 + 0 + 0) + 1 + 0) + (1 + 0 + 0) + (1)
        -> f1(2)
            -> f1(1)
                -> f1(0)
                    <- 1
                -> f1(-1)
                    <- 0
                -> f1(-2)
                    <- 0
                <- 1 + 0 + 0
            -> f1(0)
                <- 1
            -> f1(-1)
                <- 0
            <- (1 + 0 + 0) + 1 + 0
        -> f1(1)
            -> f1(0)
                <- 1
            -> f1(-1)
                <- 0
            -> f1(-2)
                <- 0
            <- 1 + 0 + 0
        <- (((1 + 0 + 0) + 1 + 0) + (1 + 0 + 0) + (1)) + ((1 + 0 + 0) + 1 + 0) + (1 + 0 + 0)
    -> f1(3)
        -> f1(2)
            -> f1(1)
                -> f1(0)
                    <- 1
                -> f1(-1)
                    <- 0
                -> f1(-2)
                    <- 0
                <- 1 + 0 + 0
            -> f1(0)
                <- 1
            -> f1(-1)
                <- 0
            <- (1 + 0 + 0) + 1 + 0
        -> f1(1)
            -> f1(0)
                <- 1
            -> f1(-1)
                <- 0
            -> f1(-2)
                <- 0
            <- 1 + 0 + 0
        -> f1(0)
            <- 1
        <- ((1 + 0 + 0) + 1 + 0) + (1 + 0 + 0) + (1)
    -> f1(2)
        -> f1(1)
            -> f1(0)
                <- 1
            -> f1(-1)
                <- 0
            -> f1(-2)
                <- 0
            <- 1 + 0 + 0
        -> f1(0)
            <- 1
        -> f1(-1)
            <- 0
        <- (1 + 0 + 0) + 1 + 0
    <- ((((1 + 0 + 0) + 1 + 0) + (1 + 0 + 0) + (1)) + ((1 + 0 + 0) + 1 + 0) + (1 + 0 + 0)) + (((1 + 0 + 0) + 1 + 0) + (1 + 0 + 0) + (1)) + ((1 + 0 + 0) + 1 + 0) = 13

### Problem 2
>
```java
public static int f2(int N) {
    if (N <= 1) {
        return 1;
    }

    int total = 0;
    for (int i = 0; i < N; i++) {
        total += f2(i) * f2(N-i-1);
    }        
    return total;
}
```

#### Desired Outputs
##### f2(3)
>
f2(3)
    // i = 0
    -> f2(0)
        <- 1
    -> f2(2)
        // i = 0
        -> f2(0)
            <- 1
        -> f2(1)
            <- 1
        
        // i = 1
        -> f2(1)
            <- 1
        -> f2(0)
            <- 1
        <- (1 * 1) + (1 * 1) = 2
    <- (1 * 2) = 2

    // i = 1
    -> f2(1)
        <- 1
    -> f2(1)
        <- 1
    <- (1 * 1)
    
    // i = 2
    -> f2(2)
        // i = 0
        -> f2(0)
            <- 1
        -> f2(1)
            <- 1
        
        // i = 1
        -> f2(1)
            <- 1
        -> f2(0)
            <- 1
        <- (1 * 1) + (1 * 1) = 2
    -> f2(0)
        <- 1
    <- (2 * 1)
<- (2) + (1) + (2) = 5

##### f2(4)
>
f2(4)
    // i = 0
    -> f2(0)
        <- 1
    -> f2(3)
        <- 5 (from the graph of above)
    <- (1 * 5) = 5

    // i = 1
    -> f2(1)
        <- 1
    -> f2(2)
        // i = 0
        -> f2(0)
            <- 1
        -> f2(1)
            <- 1
        
        // i = 1
        -> f2(1)
            <- 1
        -> f2(0)
            <- 1
        <- (1 * 1) + (1 * 1) = 2
    <- (1 * 2) = 2
    
    // i = 2
    -> f2(2)
        // i = 0
        -> f2(0)
            <- 1
        -> f2(1)
            <- 1
        
        // i = 1
        -> f2(1)
            <- 1
        -> f2(0)
            <- 1
        <- (1 * 1) + (1 * 1) = 2
    -> f2(1)
        <- 1
    <- (2 * 1) = 2
    
    // i = 3
    -> f2(3)
        <- 5 (from the graph above)
    -> f2(0)
        <- 1
    <- (5 * 1) = 5
<- 5 + 2 + 2 + 5 = 14